src/Pipit.System.Exp.fst
@@ -35,10 +35,10 @@ let rec state_of_exp (e: exp 'c 'a): Tot Type (decreases e) =
   | XMu _ e1 -> state_of_exp e1
   | XLet b e1 e2 -> state_of_exp e1 & state_of_exp e2
   // Contracts do not expose their body, so we only need state of assume, guarantee and arg
-  | XContract assm guar body arg ->
-    state_of_exp assm &
-    state_of_exp guar &
-    state_of_exp arg
+  // | XContract assm guar body arg ->
+  //   state_of_exp assm &
+  //   state_of_exp guar &
+  //   state_of_exp arg
   | XCheck name e1 e2 -> (xprop & state_of_exp e1) & state_of_exp e2
 
 let sem_freevars = (#a: Type) -> (x: C.var a) -> a
@@ -85,7 +85,7 @@ let rec dsystem_of_exp (e: exp 'c 'a)
       let t' = dsystem_mu_causal #(C.row 'c) #('a & C.row 'c) (fun i v -> (v, i)) t1 in
       Some t'
     | _ -> None)
-  | XContract assm guar body arg -> None
+  // | XContract assm guar body arg -> None
 
 let rec system_of_exp (e: exp 'c 'a)
     (fv: sem_freevars):
@@ -111,11 +111,11 @@ let rec system_of_exp (e: exp 'c 'a)
       system_mu #(C.row 'c) #('a & C.row 'c) (fun i v -> (v, i)) t
     | XLet b e1 e2 ->
       system_let (fun i v -> (v, i)) (system_of_exp e1 fv) (system_of_exp e2 fv)
-    | XContract assm guar body arg ->
-      system_contract_instance (fun i b -> (b, ())) (fun i a b -> (a, (b, ())))
-        (system_bool_holds (system_of_exp assm fv))
-        (system_bool_holds (system_of_exp guar fv))
-        (system_of_exp arg fv)
+    // | XContract assm guar body arg ->
+    //   system_contract_instance (fun i b -> (b, ())) (fun i a b -> (a, (b, ())))
+    //     (system_bool_holds (system_of_exp assm fv))
+    //     (system_bool_holds (system_of_exp guar fv))
+    //     (system_of_exp arg fv)
     | XCheck name e1 e2 ->
       let t1 = system_check name (system_of_exp e1 fv) in
       let t2 = system_of_exp e2 fv in
